WIP... complex

demo/fib/FibS2.v
@@ -15,21 +15,9 @@ Set Implicit Arguments.
 
 
 
-Fixpoint taus {E R} (n: nat) (it: itree E R): itree E R :=
-  match n with
-  | O => it
-  | S m => tau;; (taus m it)
-  end
-.
-
-Notation "n taus;; t2" := (taus n t2)
-  (at level 61, right associativity) : itree_scope.
-
 Definition f_fib (oh0: owned_heap) (m0: mem) (vs0: list val):
   itree (E owned_heap) (owned_heap * (mem * val)) :=
   n <- unwrapU (parse_arg oh0 m0 vs0) ;;
-  x <- trigger (EChoose nat) ;;
-  x taus;;
   Ret (oh0, (m0, Vint (of_nat (fib_nat n))))
 .
 
