demo/fib/FibS02proof_eutt.v
@@ -1,0 +1,151 @@
+Require Import CoqlibC Maps Postorder.
+Require Import AST Linking.
+Require Import ValuesC MemoryC GlobalenvsC Events Smallstep.
+Require Import Op ClightC.
+Require Import CtypesC CtypingC.
+Require Import sflib.
+Require Import IntegersC.
+
+Require Import Simulation.
+Require Import Skeleton Mod ModSem SimMod SimModSemLift SimSymb SimMemLift MatchSimModSemExcl.
+Require SoundTop.
+Require SimMemId.
+Require Import Any.
+Require Import SIR.
+Require Import FibHeader.
+Require Import FibS0.
+Require Import FibS2.
+Require Import ModSemProps.
+Require Import Program.
+Require Import SIRProps.
+
+Set Implicit Arguments.
+
+
+Lemma interp_mrec_bind: forall (D E : Type -> Type) (ctx : forall T : Type, D T -> itree (D +' E) T) 
+                               (U T : Type) (t : itree (D +' E) U) (k : U -> itree (D +' E) T),
+    interp_mrec ctx (` x : _ <- t;; k x) = ` x : U <- interp_mrec ctx t;; interp_mrec ctx (k x)
+.
+Proof.
+  ii. f. eapply interp_mrec_bind.
+Qed.
+
+
+
+Lemma unfold_fib: forall oh0 m0 vs0,
+    (interp_mrec (interp_function FibS0.prog) (FibS0.f_fib oh0 m0 vs0))
+      ≈
+      (`n: nat <- (unwrapU (parse_arg oh0 m0 vs0)) ;;
+    match n with
+    | O => Ret (oh0, (m0, (Vint Int.zero)))
+    | S O => Ret (oh0, (m0, (Vint Int.one)))
+    | S (S m) =>
+      let vs0 := [Vint (of_nat m)] in
+      guarantee (parse_arg oh0 m0 vs0) ;;
+      '(oh1, (m1, y1)) <- (interp_mrec (interp_function FibS0.prog) (FibS0.f_fib oh0 m0 vs0)) ;;
+
+      let vs1 := [Vint (of_nat (S m))] in
+      guarantee (parse_arg oh1 m1 vs1) ;;
+      '(oh2, (m2, y2)) <-  (interp_mrec (interp_function FibS0.prog) (FibS0.f_fib oh1 m1 vs1)) ;;
+
+      Ret (oh2, (m2, Vint (of_nat (fib_nat n))))
+    end
+      )
+.
+Proof.
+  {
+    i. irw.
+    unfold FibS0.f_fib at 2. irw.
+    unfold unwrapU. des_ifs; cycle 1.
+    { unfold triggerUB. irw. ITreelib.f_equiv. ii. ss. }
+    irw. destruct n.
+    { irw. refl. }
+    destruct n.
+    { irw. refl. }
+    destruct (to_nat_opt (of_nat n)) eqn:T; ss; cycle 1.
+    { unfold guarantee. des_ifs_safe. irw. unfold triggerNB. irw. ITreelib.f_equiv. ii; ss. }
+    unfold guarantee. des_ifs_safe. irw. rewrite tau_eutt.
+    des_ifs_safe.
+    rewrite <- ! unfold_interp_mrec.
+    rewrite interp_mrec_bind. ITreelib.f_equiv.
+    (*** TODO: I just want to use "f_equiv". The problem here is that I added
+`Require Import Morphisms.` after importing `ITreelib`.
+Solution is to import `Morphisms` inside ITreelib.
+***)
+    { refl. }
+    ii. des_ifs; cycle 1.
+    { irw. unfold triggerNB. irw. ITreelib.f_equiv. ii; ss. }
+    rewrite ! bind_ret_l.
+    rewrite interp_mrec_bind. ITreelib.f_equiv.
+    { irw. rewrite tau_eutt. des_ifs. refl. }
+    { ii. des_ifs. irw. refl. }
+  }
+Qed.
+
+
+
+Goal forall oh0 m0 vs0,
+    (interp_mrec (interp_function prog) (f_fib oh0 m0 vs0)) ≈
+    (interp_mrec (interp_function FibS0.prog) (FibS0.f_fib oh0 m0 vs0))
+.
+Proof.
+  ii.
+  destruct (parse_arg oh0 m0 vs0) eqn:T; cycle 1.
+  { unfold f_fib, FibS0.f_fib. ss.
+    unfold unwrapU. des_ifs. unfold triggerUB. irw. r.
+    ITreelib.f_equiv. ii. ss. (*** !!!!!!!!!!!!!!!!!!!!!!!!!!!!!!!!!!!!!!!!!!!!!!!!!!!!!!!! nice ***)
+  }
+  move n at top. revert_until n.
+  pattern n. eapply well_founded_ind.
+  { eapply lt_wf. }
+  clear n. intros.
+  rename x into n.
+  destruct n; ss.
+  { unfold parse_arg in *. des_ifs. unfold f_fib, FibS0.f_fib. ss. r. rewrite T. ss. irw. refl. }
+  destruct n.
+  { unfold parse_arg in *. des_ifs. unfold f_fib, FibS0.f_fib. ss. r. rewrite T. ss. irw. refl. }
+  unfold parse_arg in T. des_ifs.
+  rewrite unfold_fib. unfold unwrapU, parse_arg. rewrite T. ss. rewrite bind_ret_l.
+  assert(U: to_nat_opt (of_nat n) = Some n).
+  { admit "should be derived from guarantee". }
+  unfoldr guarantee. rewrite U. ss. des_ifs_safe. rewrite bind_ret_l.
+  assert(V: to_nat_opt (of_nat (S n)) = Some (S n)).
+  { admit "should be derived from guarantee". }
+  des_ifs. unfold guarantee. rewrite V. ss. des_ifs.
+
+
+  unfold f_fib. unfold unwrapU. rewrite unfold_interp_mrec. ss. des_ifs. rewrite ! bind_ret_l. ss.
+  rewrite <- H; cycle 1.
+  { instantiate (1:= n). eauto. }
+  { ss. }
+  unfold f_fib. unfold unwrapU. rewrite unfold_interp_mrec. ss. des_ifs. repeat (rewrite bind_ret_l; ss).
+  rewrite <- H; cycle 1.
+  { instantiate (1:= S n). eauto. }
+  { ss. }
+  unfold f_fib. ss. unfold unwrapU. des_ifs. ss. rewrite bind_ret_l.
+  rewrite unfold_interp_mrec. ss. rewrite bind_ret_l.
+  refl.
+Qed.
+
+Theorem correct: rusc defaultR [FibS2.module: Mod.t] [FibS0.module: Mod.t].
+Proof.
+  eapply SIREutt.correct; ss.
+  ii. clarify. rr.
+  unfold FibS0.prog in *. ss. des_ifs.
+  ii. clarify.
+  rename y into oh0. rename y0 into m0. rename y1 into vs0.
+  destruct (parse_arg oh0 m0 vs0) eqn:T; cycle 1.
+  { unfold f_fib, FibS0.f_fib. ss.
+    unfold unwrapU. des_ifs. unfold triggerUB. irw. r.
+    ITreelib.f_equiv. ii. ss. (*** !!!!!!!!!!!!!!!!!!!!!!!!!!!!!!!!!!!!!!!!!!!!!!!!!!!!!!!! nice ***)
+  }
+  ginduction n; ii; ss.
+  { unfold parse_arg in *. des_ifs. unfold f_fib, FibS0.f_fib. ss. r. rewrite T. ss. irw. refl. }
+  destruct n.
+  { unfold parse_arg in *. des_ifs. unfold f_fib, FibS0.f_fib. ss. r. rewrite T. ss. irw. refl. }
+  unfold parse_arg in T. des_ifs.
+  unfold f_fib, FibS0.f_fib. ss. r. rewrite T. ss. irw.
+  assert(U: to_nat_opt (of_nat n)).
+  { admit "should be derived from guarantee". }
+  unfoldr guarantee. des_ifs_safe. irw.
+Abort.
